src/Minimal.DICE.fst
@@ -9,21 +9,129 @@ open LowStar.BufferOps
 open Spec.Hash.Definitions
 open Hacl.Hash.Definitions
 
+open Lib.IntTypes
+
 open HWIface
 
 module I  = FStar.Integers
 module HI  = Lib.IntTypes
 
-module SHA2= Hacl.Hash.SHA2
-module SHA1= Hacl.Hash.SHA1
-module MD5 = Hacl.Hash.MD5
-module HMAC= Hacl.HMAC
+module SHA2       = Hacl.Hash.SHA2
+module SHA1       = Hacl.Hash.SHA1
+module MD5        = Hacl.Hash.MD5
+module HMAC       = Hacl.HMAC
+module Ed25519    = Hacl.Ed25519
+// module Curve25519 = Hacl.Curve25519
 
+(* NOTE: Hash and HMAC are using LowStar.Buffer, while Ed25519 is using Lib.Buffer *)
 module B   = LowStar.Buffer
+module LB  = Lib.Buffer
 module M   = LowStar.Modifies
 module HS  = FStar.HyperStack
 module HST = FStar.HyperStack.ST
 module IB  = LowStar.ImmutableBuffer
+// module Seq = Lib.Sequence
+
+/// <><><><><><><><><><><><> RIoT Loader Interface <><><><><><><><><><><><><>
+let version_number_t = pub_uint32
+(* NOTE: `Hacl.Ed25519` uses their own `Lib.Sequence`, `Lib.Buffer`, etc., but `Hacl.Hash.*` doesn't *)
+let signature_t = LB.lbuffer uint8 64ul
+let publickey_t = LB.lbuffer uint8 32ul
+let secretkey_t = LB.lbuffer uint8 32ul
+let msg_len_t = a:size_t{v a + 64 <= max_size_t}
+assume val riot_header_len: a:size_t{0 < v a /\ v a <= max_input_length SHA2_512}
+let raw_rheader_t = LB.lbuffer uint8 riot_header_len
+
+(* EXTENDED riot header
+   prefix `rh` for "RIoT Header" and
+   prefix `rb` for "RIoT Binary" *)
+noeq
+type riot_exheader_t = {
+     (* actual entries in headers*)
+     rversion  : version_number_t;
+     rbsize    : riot_size_t;
+     rbhash    : digest_t;
+     rhsig     : signature_t;
+     (* extra entries for convenience *)
+     rhraw     : raw_rheader_t
+  }
+
+noeq
+type riot_t = {
+  rsize   : riot_size_t;
+  rbinary : b:B.buffer uint8{B.length b == v rsize \/ b == B.null}
+  }
+
+let rcontains (h:HS.mem) (rheader: riot_exheader_t) =
+  B.live h rheader.rbhash /\
+  LB.live h rheader.rhsig /\
+  LB.live h rheader.rhraw
+
+let get_rheader_loc_l rheader = [B.loc_buffer rheader.rbhash
+                                ;LB.loc rheader.rhsig
+                                ;LB.loc rheader.rhraw]
+
+let load_rheader (_:unit)
+  (* NOTE: allocate on caller's stack *)
+: HST.StackInline (rheader: riot_exheader_t)
+  (requires fun h ->
+    (* FIXME: maintain disjointness is troublesome since I allocated different
+              buffers in different functions.
+              I didn't pass other buffers in and maintain disjointness for now.
+              I'll come back and find a better way. *)
+    True)
+  (ensures fun h0 rheader h1 ->
+    B.modifies B.loc_none h0 h1 /\
+    h1 `rcontains` rheader /\
+    B.all_disjoint (get_rheader_loc_l rheader))
+=
+  let rversion = uint #U32 #PUB 1 in
+  let rbsize   = 100ul in
+  let rbhash   = B.alloca (u8 0x00) digest_len in
+  let rhsig    = LB.create 64ul (u8 0x00) in
+  let rhraw    = LB.create riot_header_len (u8 0x00) in
+  {rversion = rversion; rbsize = rbsize; rbhash = rbhash; rhsig = rhsig; rhraw = rhraw}
+
+let verify_header
+  (rheader: riot_exheader_t)
+  (rhpubkey: publickey_t)
+: HST.StackInline bool
+  (requires fun h ->
+    h `rcontains` rheader /\
+    LB.live h rhpubkey
+    (* FIXME: maintain disjointness is troublesome since I allocated different buffers in different functions.
+              I just forget it for now. I'll come back and find a better way. *)
+    // B.all_disjoint ((get_rheader_loc_l rheader)@[LB.loc rhpubkey])
+    )
+  (ensures  fun h0 b h1 -> True)
+    (* FIXME: I haven't find the compatible SHA2 512 hash spec for Ed25519,
+              since hash uses Seq and Ed25519 uses Lib.Sequence in HALC*.
+              I believe there is a way and I will fix this tomorrow *)
+    // let rheader_hash = Spec.Agile.Hash.hash alg (LB.as_seq h0 rheader.rhraw) in
+    // b == Spec.Ed25519.verify (LB.as_seq h0 rhpubkey) rheader_hash (LB.as_seq h0 rheader.rhsig))
+=
+  let rheader_hash = LB.create 64ul (u8 0x00) in
+  SHA2.hash_512_lib riot_header_len rheader.rhraw rheader_hash;
+  Ed25519.verify rhpubkey 64ul rheader_hash rheader.rhsig
+
+(* Duties:
+   1. load RIoT header
+   2. authenticate RIoT header
+   3. load RIoT binary *)
+let load_riot
+  (rhpubkey: publickey_t)
+: HST.StackInline (riot: riot_t)
+  (requires fun h ->
+    LB.live h rhpubkey)
+  (ensures  fun h0 riot h1 ->
+    B.live h1 riot.rbinary)
+=
+  let rheader = load_rheader () in
+  if (verify_header rheader rhpubkey)
+  then (* succeed *)
+    {rsize = rheader.rbsize; rbinary = B.alloca (u8 0x00) rheader.rbsize}
+  else (* failed *)
+    {rsize = rheader.rbsize; rbinary = B.null}
 
 /// <><><><><><><><><><><><> DICE helpers <><><><><><><><><><><><><>
 
@@ -43,102 +151,15 @@ let dice_hmac (alg: dice_alg): HMAC.compute_st alg =
   | SHA2_512 -> HMAC.compute_sha2_512
   | SHA1     -> HMAC.legacy_compute_sha1
 
-(* draft spec of public sequence to secret list conversion *)
-let pub_to_sec_spec
-  (size: I.uint_32{I.v size > 0})
-  (#t: HI.inttype)
-  (seq_pub: Seq.seq HI.(int_t t PUB){Seq.length seq_pub == I.v size})
-  (seq_sec: Seq.seq HI.(int_t t SEC){Seq.length seq_sec == I.v size})
-=
-  let seq_of_size_pub = Seq.slice seq_pub 0 (I.v size - 1) in
-  let l_of_size_pub = Seq.seq_to_list seq_of_size_pub in
-  let l_of_size_sec = List.mapT HI.(fun (s:int_t t PUB) -> cast t SEC s) l_of_size_pub in
-  Seq.seq_of_list l_of_size_sec == seq_sec
-
-(* NEWLY defined mapping function without list *)
-(* This seems fine, haven't tried in `dice_main` *)
-(* NOTE: casting function for sec u8 to pub u8 is
-   NOTE: `HI.(cast #U8 #PUB U8 SEC)` *)
-let rec buffer_map_without_list
-  (size: I.uint_32)
-  (#t1 #t2: Type)
-  (f: t1 -> t2)
-  (b1: B.buffer t1{B.length b1 >= I.v size})
-  (b2: B.buffer t2{B.length b2 >= I.v size})
-: HST.Stack unit
-  (requires fun h ->
-    B.live h b1 /\
-    B.live h b2
-    (* no disjointness because it's ok to do something inplace *))
-  (ensures  fun h0 _ h1 ->
-    I.v size == 0 ==>
-      B.modifies B.loc_none h0 h1 /\
-    I.v size =!= 0 ==>
-     (B.modifies (B.loc_buffer b2) h0 h1 /\
-      List.mapT f (Seq.seq_to_list (Seq.slice (B.as_seq h0 b1) 0 (I.v size - 1)))
-               == (Seq.seq_to_list (Seq.slice (B.as_seq h1 b2) 0 (I.v size - 1)))))
-=
-  match size with
-  | 0ul -> ()
-  |  _  -> let iterator = I.(size - 1ul) in
-          let hd1 = B.index b1 iterator in
-          B.upd b2 iterator (f hd1);
-          buffer_map_without_list iterator f b1 b2
-
-(* mapping function for the first `size` elements of a buffer, which returns a list as result *)
-(* to avoid list and seq in computational code, I could rewrite it  *)
-let rec buffer_map_l
-  (size: I.uint_32)
-  (#t1 #t2: Type)
-  (f: t1 -> t2)
-  (b1: B.buffer t1{B.length b1 >= I.v size})
-: HST.StackInline (l2: list t2{List.length l2 == I.v size})
-  (requires fun h ->
-    B.live h b1)
-  (ensures  fun h0 l2 h1 ->
-    B.modifies B.loc_none h0 h1 /\
-    I.v size == 0 ==> l2 == Nil /\
-    I.v size =!= 0 ==>
-        List.mapT f (Seq.seq_to_list (Seq.slice (B.as_seq h0 b1) 0 (I.v size - 1))) == l2)
-    (decreases size)
-=
-  match size with
-  | 0ul -> Nil
-  |  _  -> let iterator = I.(size - 1ul) in
-          let hd1 = (B.index b1 iterator) in
-          let hd2 = f hd1 in
-          let tl2 = buffer_map_l iterator f b1 in
-          hd2 :: tl2
-
-(* mapping function for the first `size` elements of a buffer, which uses `buffer_map_l` and returns a newly allocated buffer on caller's stack *)
-(*
-let buffer_map
-  (size: I.uint_32{I.v size > 0})
-  (#t1 #t2: Type)
-  (f: t1 -> t2)
-  (b1: B.buffer t1{B.length b1 >= I.v size})
-: HST.StackInline (b2: B.buffer t2{B.length b2 == I.v size})
-  (requires fun h ->
-    B.live h b1)
-  (ensures  fun h0 b2 h1 ->
-    B.modifies B.loc_none h0 h1 /\
-    B.live h1 b2 /\
-    List.mapT f (Seq.seq_to_list (Seq.slice (B.as_seq h0 b1) 0 (I.v size - 1))) == Seq.seq_to_list (Seq.slice (B.as_seq h1 b2) 0 (I.v size - 1)))
-=
-  let l2: list _ = buffer_map_l size f b1 in
-  let b2 = B.alloca_of_list l2 in
-  b2
-*)
-
 /// <><><><><><><><><><><><> DICE main funtion <><><><><><><><><><><>
 
 (* This old version `dice_on_stack` is for reference purpose, not what we want finally *)
 (* F* warns when set `--query_stats` *)
 #reset-options "--z3rlimit 30 --query_stats"
-let dice_on_stack
+let dice_main
   (st: state)
   (riot_size: riot_size_t)
-  (riot_binary: B.buffer HI.uint8{B.length riot_binary == I.v riot_size})
+  (riot_binary: B.buffer uint8{B.length riot_binary == v riot_size})
 : HST.Stack unit
   (requires fun h ->
     h `HWIface.contains` st /\
@@ -161,9 +182,9 @@ let dice_on_stack
 
   (* compute uDigest *)
   let uDigest: b:B.buffer HI.uint8{B.length b == hash_length alg}
-    = B.alloca (HI.u8 0x00) digest_length in
+    = B.alloca (HI.u8 0x00) digest_len in
   dice_hash alg
-    uds uds_length
+    uds uds_len
     uDigest;
 
   (**)let h1 = HST.get () in
@@ -172,7 +193,7 @@ let dice_on_stack
 
   (* compute rDigest *)
   let rDigest: b:B.buffer HI.uint8{B.length b == hash_length alg}
-    = B.alloca (HI.u8 0x00) digest_length in
+    = B.alloca (HI.u8 0x00) digest_len in
   dice_hash alg
     riot_binary riot_size
     rDigest;
@@ -182,59 +203,11 @@ let dice_on_stack
   (**)        B.as_seq h2 rDigest == Spec.Agile.Hash.hash alg (B.as_seq h1 riot_binary));
 
   (* compute cdi *)
+  (**)assert_norm (Spec.Agile.HMAC.keysized alg (v digest_len));
   dice_hmac alg
     cdi
-    uDigest digest_length
-    rDigest digest_length;
-
-  HST.pop_frame()
-
-(* This function is under working *)
-(* I tried to use pub_uint8 buffer here and encountered many problems *)
-(* I believe lots of these problems come from `Spec.Agile.HMAC.hmac` (used in our assertions and HACL functions), which used `pow2` in its precondition `keysized` *)
-(* As we discussed, I should use `assert_norm` or some normalize ways to reduce `pow2` in F* *)
-(* Now it is a mess *)
-let dice_main
-  (st: state)
-  (riot_size: riot_size_t)
-  (* here should be HI.pub_uint8 *)
-  (riot_binary: B.buffer HI.uint8{B.length riot_binary == I.v riot_size})
-: HST.Stack unit
-  (requires fun h ->
-    h `HWIface.contains` st /\
-    h `B.live` riot_binary /\
-    B.all_disjoint ((get_loc_l st)@[B.loc_buffer riot_binary]))
-  (ensures  fun h0 _ h1 ->
-    (let uds, cdi = get_uds st, get_cdi st in
-     // let riot_binary_sec_l = pub_seq_to_sec_l_of_pos_size_spec riot_size (B.as_seq h0 riot_binary) in
-       B.modifies (B.loc_buffer cdi) h0 h1 /\
-       B.as_seq h1 cdi
-         == Spec.Agile.HMAC.hmac alg
-              (Spec.Agile.Hash.hash alg (B.as_seq h0 uds))
-              (Spec.Agile.Hash.hash alg (B.as_seq h0 riot_binary))))
-=
-  HST.push_frame();
-  let uds, cdi = get_uds st, get_cdi st in
-
-  // (**)let h0 = HST.get () in
-  let uDigest: b:B.buffer HI.uint8{B.length b == I.v digest_length} = B.alloca (HI.u8 0x00) digest_length
-  in dice_hash alg uds uds_length uDigest;
-  // (**)let h1 = HST.get () in
-  // (**)assert (B.modifies (B.loc_buffer uDigest) h0 h1 /\
-  // (**)        B.as_seq h1 uDigest == Spec.Agile.Hash.hash alg (B.as_seq h0 uds));
-
-     (* here should allocate a secret riot_binary buffer *)
-  // let riot_binary_sec = buffer_map riot_size HI.(cast #U8 #PUB U8 SEC) riot_binary in
-  // (**)let h1 = HST.get () in
-  let rDigest: b:B.buffer HI.uint8{B.length b == I.v digest_length} = B.alloca (HI.u8 0x00) digest_length
-  in dice_hash alg riot_binary riot_size rDigest;
-  // (**)let h2 = HST.get () in
-  // (**)assert (B.modifies B.(loc_buffer rDigest) h1 h2 /\
-  // (**)        B.as_seq h2 rDigest == Spec.Agile.Hash.hash alg (B.as_seq h1 riot_binary_sec));
-  // (**)assert (Spec.Agile.HMAC.keysized alg (Seq.length (B.as_seq h2 uDigest)));
-  (**)let h2 = HST.get () in
-  (**)assert_norm (Spec.Agile.HMAC.keysized alg (Seq.length (B.as_seq h2 uDigest)));
-  dice_hmac alg cdi uDigest digest_length rDigest digest_length;
+    uDigest digest_len
+    rDigest digest_len;
 
   HST.pop_frame()
 
@@ -243,10 +216,11 @@ let dice_main
 assume val riot_size: riot_size_t
 
 assume val riot_binary:
-  b:B.buffer HI.pub_uint8
-    {B.length b == I.v riot_size /\
+  b:B.buffer uint8
+    {B.length b == v riot_size /\
     (let (| _, _, local_st |) = local_state in
       B.loc_disjoint (B.loc_buffer b) (B.loc_mreference local_st))}
+
 
 let main ()
 : HST.ST C.exit_code
